iris_system/sProp.v
@@ -38,14 +38,16 @@ End HRA.
 
 Coercion HRA.subG_map: HRA.subG >-> Funclass.
 
-Module GTyp.
+(* Note that the types in a group has the type PF.t *)
 
-  Class t: Type := __GTYP : GPF.t.
+(* The types in all groups *)
+Module Typ.
 
-End GTyp.
+  Class t: Type := __TYP : GPF.t.
 
+End Typ.
 
-(** Types **)
+(** Types for Separation Logic **)
 
 Module ST.
 
@@ -85,7 +87,7 @@ End ST.
 
 Module CtxST.
 
-  Class t `{τ: GTyp.t}
+  Class t `{τ: Typ.t}
     `{_C: @GPF.inG ST.t τ}
     := ctxSL: unit.
 
@@ -103,11 +105,13 @@ Infix "+" := (ST.sumT) : SRF_scope.
 Notation "'τ{' t ',' n '}'" := (@PF.deg ST.t t (SRFSyn.t_prev n)) : SRF_scope.
 Notation "'τ{' t '}'" := (@PF.deg ST.t t (SRFSyn.t_prev _)) : SRF_scope.
 
+(* Separation Logic *)
+
 Module SL.
 
   Section SL.
 
-  Context `{τ: GTyp.t}.
+  Context `{τ: Typ.t}.
   Context `{Γ: HRA.t}.
   
   Variant shape : Type :=
@@ -116,8 +120,8 @@ Module SL.
     | _and
     | _or
     | _impl
-    | _univ i (ty : τ i)
-    | _ex   i (ty : τ i)
+    | _univ i (ty : (τ i).(PF.shp))
+    | _ex   i (ty : (τ i).(PF.shp))
     | _empty
     | _sepconj
     | _wand
@@ -133,8 +137,8 @@ Module SL.
     | _and => fin 2
     | _or => fin 2
     | _impl => fin 2
-    | _univ i ty => PF.deg ty Prev
-    | _ex   i ty => PF.deg ty Prev
+    | _univ i ty => (τ i).(PF.deg) ty Prev
+    | _ex   i ty => (τ i).(PF.deg) ty Prev
     | _empty => fin 0
     | _sepconj => fin 2
     | _wand => fin 2
@@ -148,12 +152,11 @@ Module SL.
       deg := degree;
     }.
 
-  Context `{α: @SRFMSynG.t}.
+  Context `{α: @SRFCons.t}.
   Context `{_C0: @HRA.subG Γ Σ}.
   
   Global Instance domain : SRFDom.t := {
     dom := iProp;
-    void := False%I;
   }.
   
   Definition interp n (s: shape) : (degree s (SRFSyn.t_prev n) -> SRFSyn.t n) -> (degree s (SRFSyn.t_prev n) -> iProp) -> iProp :=
@@ -173,9 +176,9 @@ Module SL.
     | _upd => fun _ sem => Upd (sem 0%fin)
     end.
 
-  Global Instance t: SRFMSem.t := interp.
+  Global Instance t: SRFIntpM.t := interp.
 
-  Context `{@SRFMSemG.inG _ _ _ t β}.
+  Context `{@SRFIntp.inG _ _ _ t β}.
   
   Definition ownm `{IN: @GRA.inG M Γ} {n} (r: M) : SRFSyn.t n.
     destruct IN. subst.
@@ -209,12 +212,12 @@ Module SL.
     - exact p2.
   Defined.
   
-  Definition univ `{IN: @GPF.inG T τ} {n} (ty:T) (p: PF.deg ty (SRFSyn.t_prev n) -> SRFSyn.t n) : SRFSyn.t n.
+  Definition univ `{IN: @GPF.inG T τ} {n} (ty: T.(PF.shp)) (p: T.(PF.deg) ty (SRFSyn.t_prev n) -> SRFSyn.t n) : SRFSyn.t n.
     destruct IN. subst.
     exact ⟨ _univ _ ty, p ⟩%SRF.
   Defined.
 
-  Definition ex `{IN: @GPF.inG T τ} {n} (ty: T) (p: PF.deg ty (SRFSyn.t_prev n) -> SRFSyn.t n) : SRFSyn.t n.
+  Definition ex `{IN: @GPF.inG T τ} {n} (ty: T.(PF.shp)) (p: T.(PF.deg) ty (SRFSyn.t_prev n) -> SRFSyn.t n) : SRFSyn.t n.
     destruct IN. subst.
     exact ⟨ _ex _ ty, p ⟩%SRF.
   Defined.
@@ -285,10 +288,10 @@ End SL.
 
 Module CtxSL.
 
-  Class t `{Γ: HRA.t} `{Σ: GRA.t} `{α: SRFMSynG.t} `{β: @SRFMSemG.t SL.domain α}
+  Class t `{Γ: HRA.t} `{Σ: GRA.t} `{α: SRFCons.t} `{β: @SRFIntp.t SL.domain α}
     `{_C: CtxST.t}
     `{_C: @HRA.subG Γ Σ}
-    `{_C: @SRFMSemG.inG SL.domain _ α SL.t β}
+    `{_C: @SRFIntp.inG SL.domain _ α SL.t β}
     := ctxSL: unit.
   
 End CtxSL.
@@ -374,7 +377,7 @@ Module SLRed.
     SRFSem.t n (SL.impl p q) = (SRFSem.t n p → SRFSem.t n q)%I.
   Proof. unfold SL.impl. rewrite @SRFRed.cur. reflexivity. Qed.
 
-  Lemma univ `{T:PF.t} `{@GPF.inG T τ} n (ty: T) p :
+  Lemma univ `{T:PF.t} `{@GPF.inG T τ} n (ty: T.(PF.shp)) p :
     SRFSem.t n (SL.univ ty p) = (∀ x: (T.(PF.deg) ty (SRFSyn.t_prev n)), SRFSem.t n (p x))%I.
   Proof.
     destruct H eqn: EQ. subst.
